finish pset 1

pset01_ProgramAnalysis/Pset1Implementation.v
@@ -19,16 +19,18 @@ Module Impl.
   (* Define [Neg] so that it implements Boolean negation, which flips
    * the truth value of a Boolean value.
    *)
-  Definition Neg (b : bool) : bool.
-  Admitted.
-
+  Definition Neg (b : bool) : bool :=
+    match b with
+    | true => false
+    | false => true
+    end.
+  
   (* For instance, the negation of [true] should be [false].
    * This proof should follow from reducing both sides of the equation
    * and observing that they are identical.
    *)
   Theorem Neg_true : Neg true = false.
-  Proof.
-  Admitted.
+  Proof. equality. Qed.
 
   (* Negation should be involutive, meaning that if we negate
    * any Boolean value twice, we should get the original value back.
@@ -38,40 +40,40 @@ Module Impl.
    * [cases] tactic.
    *)
   Theorem Neg_involutive : forall b : bool, Neg (Neg b) = b.
-  Proof.
-  Admitted.
+  Proof. intros b. cases b; equality. Qed.
 
   (* Define [And] so that it implements Boolean conjunction. That is,
    * the result value should be [true] exactly when both inputs
    * are [true].
    *)
-  Definition And (x y : bool) : bool.
-  Admitted.
+  Definition And (x y : bool) : bool :=
+    match x, y with
+    | true, true => true
+    | _, _ => false
+    end.
 
   (* Here are a couple of examples of how [And] should act on
    * concrete inputs.
    *)
   Theorem And_true_true : And true true = true.
-  Proof.
-  Admitted.
+  Proof. equality. Qed.
 
   Theorem And_false_true : And false true = false.
-  Proof.
-  Admitted.
+  Proof. equality. Qed.
 
   (* Prove that [And] is commutative, meaning that switching the order
    * of its arguments doesn't affect the result.
    *)
   Theorem And_comm : forall x y : bool, And x y = And y x.
   Proof.
-  Admitted.
+    intros x y. cases x; cases y; equality. Qed.
 
   (* Prove that the conjunction of a Boolean value with [true]
    * doesn't change that value.
    *)
   Theorem And_true_r : forall x : bool, And x true = x.
   Proof.
-  Admitted.
+    intros x. cases x; equality. Qed.
 
   (* In the second part of this assignment, we will work with a simple language
    * of imperative arithmetic programs that sequentially apply operations
@@ -86,43 +88,60 @@ Module Impl.
    * that running the program [p] should result in, when the
    * initial state is [n].
    *)
-  Fixpoint run (p : Prog) (initState : nat) : nat.
-  Admitted.
-
+  Fixpoint run (p : Prog) (initState : nat) : nat :=
+    match p with
+    | Done => initState
+    | AddThen n p' => run p' (initState + n)
+    | MulThen n p' => run p' (initState * n)
+    | DivThen n p' => run p' (initState / n)
+    | VidThen n p' => run p' (n / initState)
+    | SetToThen n p' => run p' n
+    end.
+  
   Theorem run_Example1 : run Done 0 = 0.
-  Proof.
-  Admitted.
+  Proof. equality. Qed.
 
   Theorem run_Example2 : run (MulThen 5 (AddThen 2 Done)) 1 = 7.
-  Proof.
-  Admitted.
+  Proof. equality. Qed.
 
   Theorem run_Example3 : run (SetToThen 3 (MulThen 2 Done)) 10 = 6.
-  Proof.
-  Admitted.
+  Proof. equality. Qed.
 
   (* Define [numInstructions] to compute the number of instructions
    * in a program, not counting [Done] as an instruction.
    *)
-  Fixpoint numInstructions (p : Prog) : nat.
-  Admitted.
-
+  Fixpoint numInstructions (p : Prog) : nat :=
+    match p with
+    | Done => 0
+    | AddThen _ p' => 1 + numInstructions p'
+    | MulThen _ p' => 1 + numInstructions p'
+    | DivThen _ p' => 1 + numInstructions p'
+    | VidThen _ p' => 1 + numInstructions p'
+    | SetToThen _ p' => 1 + numInstructions p'
+    end.
+    
+    
   Theorem numInstructions_Example :
     numInstructions (MulThen 5 (AddThen 2 Done)) = 2.
-  Proof.
-  Admitted.
+  Proof. equality. Qed.
 
   (* Define [concatProg] such that [concatProg p1 p2] is the program
    * that first runs [p1] and then runs [p2].
    *)
-  Fixpoint concatProg (p1 p2 : Prog) : Prog.
-  Admitted.
+  Fixpoint concatProg (p1 p2 : Prog) : Prog :=
+    match p1 with
+    | Done => p2
+    | AddThen n p' => AddThen n (concatProg p' p2)
+    | MulThen n p' => MulThen n (concatProg p' p2)
+    | DivThen n p' => DivThen n (concatProg p' p2)
+    | VidThen n p' => VidThen n (concatProg p' p2)
+    | SetToThen n p' => SetToThen n (concatProg p' p2)
+    end.
 
   Theorem concatProg_Example :
        concatProg (AddThen 1 Done) (MulThen 2 Done)
        = AddThen 1 (MulThen 2 Done).
-  Proof.
-  Admitted.
+  Proof. equality. Qed.
 
   (* Prove that the number of instructions in the concatenation of
    * two programs is the sum of the number of instructions in each
@@ -132,8 +151,10 @@ Module Impl.
     : forall (p1 p2 : Prog), numInstructions (concatProg p1 p2)
                         = numInstructions p1 + numInstructions p2.
   Proof.
-  Admitted.
-
+    intros p1 p2.
+    induct p1; simplify; equality.
+  Qed.
+      
   (* Prove that running the concatenation of [p1] with [p2] is
      equivalent to running [p1] and then running [p2] on the
      result. *)
@@ -142,7 +163,9 @@ Module Impl.
       run (concatProg p1 p2) initState =
       run p2 (run p1 initState).
   Proof.
-  Admitted.
+    intros p1 p2 initState.
+    induct p1; simplify; equality.
+  Qed.
 
   (* Read this definition and understand how division by zero is handled. *)
   Fixpoint runPortable (p : Prog) (state : nat) : bool * nat :=
@@ -181,11 +204,19 @@ Module Impl.
   (* Prove that running the concatenation [p] using [runPortable]
      coincides with using [run], as long as [runPortable] returns
      [true] to confirm that no divison by zero occurred. *)
+
   Lemma runPortable_run : forall p s0 s1,
     runPortable p s0 = (true, s1) -> run p s0 = s1.
   Proof.
-  Admitted.
-
+    intros p s0 s1 H.
+    induct p; simplify; try equality.
+    { apply IHp in H.
+      replace (s0 + n) with (n + s0); linear_arithmetic. }
+    { apply IHp in H.
+      replace (s0 * n) with (n * s0); linear_arithmetic. }
+    all: cases n; cases s0; simplify; try linear_arithmetic; try apply IHp in H; equality.
+  Qed.
+      
   (* The final goal of this pset is to implement [validate : Prog -> bool]
      such that if this function returns [true], the program would not trigger
      division by zero regardless of what state it starts out in.  [validate] is
@@ -220,27 +251,53 @@ Module Impl.
 
   (* HINT 1 (see Pset1Signature.v) *)
 
-  Definition validate (p : Prog) : bool.
-  Admitted.
+  Fixpoint validate' (p : Prog) (nz : bool) : bool :=
+    match p with
+    | Done => true
+    | AddThen n p' => match n with
+                      | 0 => validate' p' nz
+                      | _ => validate' p' true
+                      end
+    | MulThen n p' => match n with
+                      | 0 => validate' p' false
+                      | _ => validate' p' nz
+                      end
+    | DivThen n p' => match n with
+                      | 0 => false
+                      | 1 => validate' p' nz
+                      | _ => validate' p' false
+                      end
+    | VidThen n p' => match nz with
+                      | true => validate' p' false
+                      | false => false
+                      end
+    | SetToThen n p' => match n with
+                        | 0 => validate' p' false
+                        | _ => validate' p' true
+                        end
+    end.
+  
+  Definition validate (p : Prog) : bool :=
+    validate' p false.
 
   (* Start by making sure that your solution passes the following tests, and add
    * at least one of your own tests: *)
 
-  Example validate1 : validate goodProgram1 = true. Admitted.
-  Example validate2 : validate goodProgram2 = true. Admitted.
-  Example validate3 : validate goodProgram3 = true. Admitted.
-  Example validate4 : validate goodProgram4 = true. Admitted.
-  Example validate5 : validate goodProgram5 = true. Admitted.
-  Example validate6 : validate goodProgram6 = true. Admitted.
-  Example validate7 : validate goodProgram7 = true. Admitted.
-  Example validateb1 : validate badProgram1 = false. Admitted.
-  Example validateb2 : validate badProgram2 = false. Admitted.
+  Example validate1 : validate goodProgram1 = true. equality. Qed.
+  Example validate2 : validate goodProgram2 = true. equality. Qed.
+  Example validate3 : validate goodProgram3 = true. equality. Qed.
+  Example validate4 : validate goodProgram4 = true. equality. Qed.
+  Example validate5 : validate goodProgram5 = true. equality. Qed.
+  Example validate6 : validate goodProgram6 = true. equality. Qed.
+  Example validate7 : validate goodProgram7 = true. equality. Qed.
+  Example validateb1 : validate badProgram1 = false. equality. Qed.
+  Example validateb2 : validate badProgram2 = false. equality. Qed.
 
   (* Then, add your own example of a bad program here, and check that `validate`
    * returns `false` on it: *)
 
-  Definition badProgram3 : Prog. Admitted.
-  Example validateb3 : validate badProgram3 = false. Admitted.
+  Definition badProgram3 : Prog := AddThen 1 (DivThen 2 (SetToThen 0 (VidThen 10 Done))).
+  Example validateb3 : validate badProgram3 = false. equality. Qed.
 
   (* HINTs 2-6 (see Pset1Signature.v)  *)
 
@@ -252,13 +309,85 @@ Module Impl.
    * proceeding. *)
 
   (** Proof sketch: **)
-  (* [[Fill in your proof sketch here.]] *)
+  (* 
+(validate p' false) may depend on (validate p true) depending on what arguments are provided
+lemma needs to account for both (validate p' false) and (validate p' true)
+
+Lemma validate'_sound : forall p,
+      (validate' p true = true ->
+               forall s, (s <> 0) -> runPortable p s = (true, run p s)) /\
+      (validate' p false = true ->
+                 forall s, runPortable p s = (true, run p s)).
+
+Induct on p
+Base Case : p = Done -> trivial
+Inductive Hypothesis: Let p' = _ _ p, and assume that p satisfies validate'_sound. Then,
+  p' = AddThen n p
+     if n==0
+        If validate p true = true --> validate p' true = true
+        runPortable p' s = runPortable p (0+s) = (true, run p (0+s)) = (true, run p' s)
+        (0+s)<>0 because s<>0 by inductive hypothesis
+
+        Otherwise vadliate p false = true --> validate p' false = true
+        runPortable p' s = runPortable p (0+s) = (true, run p (0+s)) = (true, run p' s)
+     case where n<>0 follows similarly
+  p' = MulThen n p
+     runPortable p' s = runPortable p (n*s)
+     destruct into cases where n=0 and n<>0
+  p' = DivThen n p
+     runPortable p' s = runPortable p (s/n)
+     destruct into cases where n=0, n=1, n>=2
+  p' = VidThen n p
+     runPortable p' s = runPortable p (n/s)
+     destruct into cases where s=0 and s<>0
+  p' = SetToThen n p
+     runPortable p' s = runPortable p n
+     destruct into cases where n=0 and n<>0
+
+Cases should follow similarly to the case where (p' = AddThen n p) and n=0.
+   *)
 
   (* Now you're ready to write the proof in Coq: *)
 
+  Hint Rewrite plus_0_r Nat.mul_0_r Nat.div_1_r Nat.div_0_l.
+
+  Ltac arith_rewrite :=
+    match goal with
+    | [|- runPortable (?p) (?a) = (true, run (?p) (?b))] => replace (b) with (a) by linear_arithmetic
+    end.
+
+  Ltac apply_ind_hyp IHp :=
+    match goal with
+    | [H: validate' ?p true = true |- _] => apply proj1 in IHp
+    | [H: validate' ?p false = true |- _] => apply proj2 in IHp
+    end; apply IHp; try simplify; try equality; try linear_arithmetic.
+  
+  Lemma validate'_sound : forall p,
+      (validate' p true = true ->
+               forall s, (s <> 0) -> runPortable p s = (true, run p s)) /\
+      (validate' p false = true ->
+                 forall s, runPortable p s = (true, run p s)).
+  Proof.
+    intros.
+    induct p; try equality;
+      split; cases n; simplify;
+      cases (s ==n 0); try linear_arithmetic; try equality;
+      try arith_rewrite; try apply_ind_hyp IHp.
+    all: cases n; apply_ind_hyp IHp.
+      
+    (* { equality. } *)
+    (* { split; cases n; simplify; try arith_rewrite; apply_ind_hyp IHp. } *)
+    (* { split; cases n; simplify; try linear_arithmetic; try arith_rewrite; apply_ind_hyp IHp. } *)
+    (* { split; cases n; simplify; try linear_arithmetic; cases n; apply_ind_hyp IHp. } *)
+    (* { split; cases n; simplify; destruct (s ==n 0); try equality; try linear_arithmetic. } *)
+    (* { split; cases n; simplify; apply_ind_hyp IHp. } *)
+  Qed.
+        
   Lemma validate_sound : forall p, validate p = true ->
     forall s, runPortable p s = (true, run p s).
-  Admitted.
+  Proof.
+    apply validate'_sound.
+  Qed.
 
   (* Here is the complete list of commands used in one possible solution:
     - Search, for example Search (_ + 0).
